Remove HeapSig.

pulse/lib/core/PulseCore.BaseHeapSig.fsti
@@ -1,9 +1,10 @@
 module PulseCore.BaseHeapSig
-open PulseCore.HeapSig
 open FStar.Ghost
 open FStar.PCM
+module Set = FStar.GhostSet
 module H = PulseCore.Heap
 module H2 = PulseCore.Heap2
+module ST = PulseCore.HoareStateMonad
 
 type mem : Type u#(a + 1) = H2.heap u#a
 
@@ -13,16 +14,16 @@ let disjoint_mem (m0 m1: mem) : prop = H2.disjoint m0 m1
 
 let join_mem (m0:mem) (m1:mem { disjoint_mem m0 m1 }) : mem = H2.join m0 m1
 
-let sep : separable (mem u#a) = {
-    empty = empty_mem;
-    disjoint = disjoint_mem;
-    join = join_mem;
-    disjoint_sym = (fun m1 m2 -> H2.disjoint_sym m1 m2);
-    join_commutative = (fun h0 h1 -> H2.join_commutative h0 h1); 
-    disjoint_join = (fun m1 m2 m3 -> H2.disjoint_join m1 m2 m3);
-    join_associative = (fun h0 h1 h2 -> H2.join_associative h0 h1 h2);
-    join_empty = (fun m -> H2.join_empty m);
-}
+let non_info (t:Type u#a) : Type u#a = x:erased t -> (y:t { y == reveal x })
+
+let core_ref: Type u#0 = H2.core_ref
+let core_ref_null = H2.core_ref_null
+let is_null : core_ref -> GTot bool = H2.core_ref_is_null
+let ref (a:Type u#a) (p:pcm a) = core_ref
+
+let core_ghost_ref : Type u#0 = H2.core_ghost_ref
+let ghost_ref (a:Type u#a) (p:pcm a) = core_ghost_ref
+let add (#a:Type) (f:Set.decide_eq a) (x:a) (y:Set.set a) = Set.union (Set.singleton f x) y
 
 let full_mem_pred m = H2.full_heap_pred m
 
@@ -31,9 +32,16 @@ let is_ghost_action m0 m1 : prop =
 
 let slprop = H2.slprop
 
-val interp (p:slprop u#a) : affine_mem_prop u#(a+1) sep
+let is_affine_mem_prop (p:mem -> prop)
+: prop
+= forall (m0 m1:mem). p m0 /\ disjoint_mem m0 m1 ==> p (join_mem m0 m1)
 
-val as_slprop (p:affine_mem_prop sep) : q:slprop{forall h. interp q h <==> p h}
+let affine_mem_prop
+= p:(mem u#a -> prop){ is_affine_mem_prop p }
+
+val interp (p:slprop u#a) : affine_mem_prop u#a
+
+val as_slprop (p:affine_mem_prop) : q:slprop{forall h. interp q h <==> p h}
 
 let emp : slprop = H2.emp
 val pure (p:prop) : slprop
@@ -44,8 +52,8 @@ val star_equiv (p q:slprop u#a) (m:mem u#a)
 : Lemma (
     interp (p `star` q) m <==> 
         (exists m0 m1. 
-          sep.disjoint m0 m1 /\
-          m == sep.join m0 m1 /\
+          disjoint_mem m0 m1 /\
+          m == join_mem m0 m1 /\
           interp p m0 /\
           interp q m1)
   )
@@ -53,7 +61,10 @@ val star_equiv (p q:slprop u#a) (m:mem u#a)
 val slprop_extensionality (p q:slprop)
 : Lemma ((forall c. interp p c <==> interp q c) ==> p == q)
 
-val interp_as (p:affine_mem_prop sep)
+val star_commutative (p q: slprop) : Lemma (star p q == star q p)
+val star_associative p q r : Lemma (star (star p q) r == star p (star q r))
+
+val interp_as (p:affine_mem_prop)
 : Lemma (forall c. interp (as_slprop p) c == p c)
 
 val emp_unit (p:slprop) : Lemma (p == (p `star` emp))
@@ -65,29 +76,46 @@ let update_ghost (m0:mem u#a) (m1:erased (mem u#a) { is_ghost_action m0 m1 })
 val pure_true_emp () : Lemma (pure True == emp)
 val intro_emp (h:mem) : Lemma (interp emp h)
 val pure_interp (p:prop) (c:mem) : Lemma (interp (pure p) c == p)
-let base_heap : heap_sig u#a =
-  {
-    mem;
-    sep;
-    full_mem_pred;
-    is_ghost_action;
-    is_ghost_action_preorder= (fun _ -> ());
-    update_ghost;
-    slprop;
-    interp;
-    as_slprop;
-    interp_as;
-    slprop_extensionality;
-    non_info_slprop = (fun x -> reveal x);
-    emp;
-    pure;
-    star;
-    intro_emp;
-    pure_interp;
-    pure_true_emp;
-    emp_unit;
-    star_equiv;
-}
+let is_ghost_action_preorder () : Lemma (FStar.Preorder.preorder_rel is_ghost_action) = ()
+
+let full_mem  = m:mem{ full_mem_pred m }
+let maybe_ghost_action (maybe_ghost:bool) (m0 m1:mem)
+    = maybe_ghost ==> is_ghost_action m0 m1
+
+let step_t 
+  (a:Type u#a)
+  (maybe_ghost:bool)
+  (expects:slprop)
+  (provides: a -> GTot slprop)
+  (frame:slprop)
+= ST.st #(full_mem u#m) a
+    (requires fun m0 ->
+        interp (expects `star` frame) m0)
+    (ensures fun m0 x m1 ->
+        maybe_ghost_action maybe_ghost m0 m1 /\
+        interp (expects `star` frame) m0 /\  //TODO: fix the effect so as not to repeat this
+        interp (provides x `star` frame) m1)
+
+(** An action is just a thunked computation in [MstTot] that takes a frame as argument *)
+let _action_except 
+    (a:Type u#a)
+    (maybe_ghost:bool)
+    (expects:slprop u#m)
+    (provides: a -> GTot slprop)
+ : Type u#(max a (m + 1)) 
+ = frame:slprop -> step_t a maybe_ghost expects provides frame
+
+let action_except
+    (a:Type u#a)
+    (expects:slprop u#m)
+    (provides:a -> GTot slprop)
+= _action_except a false expects provides
+
+let ghost_action_except
+      (a:Type u#a)
+      (expects:slprop u#m)
+      (provides: a -> GTot slprop)
+= _action_except a true expects provides
 
 val core_ghost_ref_is_null (c:core_ghost_ref) : GTot bool
 let non_null_core_ghost_ref = r:core_ghost_ref { not (core_ghost_ref_is_null r) }
@@ -100,25 +128,25 @@ val core_ghost_ref_as_addr_injective (c1:core_ghost_ref)
 val addr_as_core_ghost_ref_injective (a:nat)
 : Lemma 
   (ensures core_ghost_ref_as_addr (addr_as_core_ghost_ref a) == a)
-val select_ghost (i:nat) (m:(base_heap u#a).mem) : GTot (option (H.cell u#a))
-val ghost_ctr (b:base_heap.mem) : GTot nat
-let free_above_ghost_ctr (m:base_heap.mem)
+val select_ghost (i:nat) (m:mem u#a) : GTot (option (H.cell u#a))
+val ghost_ctr (b:mem) : GTot nat
+let free_above_ghost_ctr (m:mem u#a)
 : prop
 = forall addr. addr >= ghost_ctr m ==> select_ghost addr m == None
 val empty_mem_props () 
 : Lemma (
-    free_above_ghost_ctr base_heap.sep.empty /\
-    ghost_ctr base_heap.sep.empty == 0
+    free_above_ghost_ctr empty_mem /\
+    ghost_ctr empty_mem == 0
   )
 
-val pts_to (#a:Type u#a) (#p:pcm a) (r:ref a p) (x:a) : (base_heap u#a).slprop
-val ghost_pts_to (#a:Type u#a) (#p:pcm a) (r:ghost_ref a p) (x:a) : (base_heap u#a).slprop
+val pts_to (#a:Type u#a) (#p:pcm a) (r:ref a p) (x:a) : slprop u#a
+val ghost_pts_to (#a:Type u#a) (#p:pcm a) (r:ghost_ref a p) (x:a) : slprop u#a
 
 val ghost_extend
     (#a:Type)
     (#pcm:pcm a)
     (x:erased a{pcm.refine x})
-: ghost_action_except base_heap (ghost_ref a pcm) emp (fun r -> ghost_pts_to r x)
+: ghost_action_except (ghost_ref a pcm) emp (fun r -> ghost_pts_to r x)
 
 val ghost_read
     (#a:Type)
@@ -128,7 +156,7 @@ val ghost_read
     (f:(v:a{compatible p x v}
         -> GTot (y:a{compatible p y v /\
                      FStar.PCM.frame_compatible p x v y})))
-: ghost_action_except base_heap (erased (v:a{compatible p x v /\ p.refine v}))
+: ghost_action_except (erased (v:a{compatible p x v /\ p.refine v}))
         (ghost_pts_to r x)
         (fun v -> ghost_pts_to r (f v)) 
 
@@ -138,7 +166,7 @@ val ghost_write
     (r:ghost_ref a p)
     (x y:Ghost.erased a)
     (f:FStar.PCM.frame_preserving_upd p x y)
-: ghost_action_except base_heap unit
+: ghost_action_except unit
         (ghost_pts_to r x)
         (fun _ -> ghost_pts_to r y)
 
@@ -148,9 +176,9 @@ val ghost_share
     (r:ghost_ref a pcm)
     (v0:FStar.Ghost.erased a)
     (v1:FStar.Ghost.erased a{composable pcm v0 v1})
-: ghost_action_except base_heap unit
+: ghost_action_except unit
     (ghost_pts_to r (v0 `op pcm` v1))
-    (fun _ -> ghost_pts_to r v0 `base_heap.star` ghost_pts_to r v1)
+    (fun _ -> ghost_pts_to r v0 `star` ghost_pts_to r v1)
 
 val ghost_gather
     (#a:Type)
@@ -158,15 +186,15 @@ val ghost_gather
     (r:ghost_ref a pcm)
     (v0:FStar.Ghost.erased a)
     (v1:FStar.Ghost.erased a)
-: ghost_action_except base_heap (squash (composable pcm v0 v1))
-    (ghost_pts_to r v0 `base_heap.star` ghost_pts_to r v1)
+: ghost_action_except (squash (composable pcm v0 v1))
+    (ghost_pts_to r v0 `star` ghost_pts_to r v1)
     (fun _ -> ghost_pts_to r (op pcm v0 v1))
 
 val extend
     (#a:Type)
     (#pcm:pcm a)
     (x:a{pcm.refine x})
-: action_except base_heap (ref a pcm) emp (fun r -> pts_to r x)
+: action_except (ref a pcm) emp (fun r -> pts_to r x)
 
 val read
     (#a:Type)
@@ -176,7 +204,7 @@ val read
     (f:(v:a{compatible p x v}
         -> GTot (y:a{compatible p y v /\
                      FStar.PCM.frame_compatible p x v y})))
-: action_except base_heap (v:a{compatible p x v /\ p.refine v})
+: action_except (v:a{compatible p x v /\ p.refine v})
     (pts_to r x)
     (fun v -> pts_to r (f v))
 
@@ -186,7 +214,7 @@ val write
     (r:ref a p)
     (x y:Ghost.erased a)
     (f:FStar.PCM.frame_preserving_upd p x y)
-: action_except base_heap unit
+: action_except unit
     (pts_to r x)
     (fun _ -> pts_to r y)
 
@@ -196,9 +224,9 @@ val share
     (r:ref a pcm)
     (v0:FStar.Ghost.erased a)
     (v1:FStar.Ghost.erased a{composable pcm v0 v1})
-: ghost_action_except base_heap unit
+: ghost_action_except unit
     (pts_to r (v0 `op pcm` v1))
-    (fun _ -> pts_to r v0 `base_heap.star` pts_to r v1)
+    (fun _ -> pts_to r v0 `star` pts_to r v1)
 
 val gather
     (#a:Type)
@@ -206,8 +234,8 @@ val gather
     (r:ref a pcm)
     (v0:FStar.Ghost.erased a)
     (v1:FStar.Ghost.erased a)
-: ghost_action_except base_heap (squash (composable pcm v0 v1))
-    (pts_to r v0 `base_heap.star` pts_to r v1)
+: ghost_action_except (squash (composable pcm v0 v1))
+    (pts_to r v0 `star` pts_to r v1)
     (fun _ -> pts_to r (op pcm v0 v1))
 
 val pts_to_not_null_action 
@@ -215,17 +243,17 @@ val pts_to_not_null_action
       (#pcm:pcm a)
       (r:erased (ref a pcm))
       (v:Ghost.erased a)
-: ghost_action_except base_heap (squash (not (is_null r)))
+: ghost_action_except (squash (not (is_null r)))
     (pts_to r v)
     (fun _ -> pts_to r v)
 
-val ghost_pts_to' (#a:Type u#a) (#p:pcm a) (r:ghost_ref a p) (x:a) : (base_heap u#(max a b)).slprop
+val ghost_pts_to' (#a:Type u#a) (#p:pcm a) (r:ghost_ref a p) (x:a) : slprop u#(max a b)
 
 val ghost_extend'
     (#a:Type u#a)
     (#pcm:pcm a)
     (x:erased a{pcm.refine x})
-: ghost_action_except base_heap (ghost_ref a pcm) emp (fun r -> ghost_pts_to' u#a u#b r x)
+: ghost_action_except (ghost_ref a pcm) emp (fun r -> ghost_pts_to' u#a u#b r x)
 
 val ghost_read'
     (#a:Type)
@@ -235,7 +263,7 @@ val ghost_read'
     (f:(v:a{compatible p x v}
         -> GTot (y:a{compatible p y v /\
                      FStar.PCM.frame_compatible p x v y})))
-: ghost_action_except base_heap (erased (v:a{compatible p x v /\ p.refine v}))
+: ghost_action_except (erased (v:a{compatible p x v /\ p.refine v}))
         (ghost_pts_to' u#a u#b r x)
         (fun v -> ghost_pts_to' u#a u#b r (f v)) 
 
@@ -245,7 +273,7 @@ val ghost_write'
     (r:ghost_ref a p)
     (x y:Ghost.erased a)
     (f:FStar.PCM.frame_preserving_upd p x y)
-: ghost_action_except base_heap unit
+: ghost_action_except unit
         (ghost_pts_to' u#a u#b r x)
         (fun _ -> ghost_pts_to' u#a u#b r y)
 
@@ -255,9 +283,9 @@ val ghost_share'
     (r:ghost_ref a pcm)
     (v0:FStar.Ghost.erased a)
     (v1:FStar.Ghost.erased a{composable pcm v0 v1})
-: ghost_action_except base_heap unit
+: ghost_action_except unit
     (ghost_pts_to' u#a u#b r (v0 `op pcm` v1))
-    (fun _ -> ghost_pts_to' u#a u#b r v0 `base_heap.star` ghost_pts_to' u#a u#b r v1)
+    (fun _ -> ghost_pts_to' u#a u#b r v0 `star` ghost_pts_to' u#a u#b r v1)
 
 val ghost_gather'
     (#a:Type)
@@ -265,17 +293,17 @@ val ghost_gather'
     (r:ghost_ref a pcm)
     (v0:FStar.Ghost.erased a)
     (v1:FStar.Ghost.erased a)
-: ghost_action_except base_heap (squash (composable pcm v0 v1))
-    (ghost_pts_to' u#a u#b r v0 `base_heap.star` ghost_pts_to' u#a u#b r v1)
+: ghost_action_except (squash (composable pcm v0 v1))
+    (ghost_pts_to' u#a u#b r v0 `star` ghost_pts_to' u#a u#b r v1)
     (fun _ -> ghost_pts_to' u#a u#b r (op pcm v0 v1))
 
-val pts_to' (#a:Type u#a) (#p:pcm a) (r:ref a p) (x:a) : (base_heap u#(max a b)).slprop
+val pts_to' (#a:Type u#a) (#p:pcm a) (r:ref a p) (x:a) : slprop u#(max a b)
 
 val extend'
     (#a:Type)
     (#pcm:pcm a)
     (x:a{pcm.refine x})
-: action_except base_heap (ref a pcm) emp (fun r -> pts_to' u#a u#b r x)
+: action_except (ref a pcm) emp (fun r -> pts_to' u#a u#b r x)
 
 val read'
     (#a:Type)
@@ -285,7 +313,7 @@ val read'
     (f:(v:a{compatible p x v}
         -> GTot (y:a{compatible p y v /\
                      FStar.PCM.frame_compatible p x v y})))
-: action_except base_heap (v:a{compatible p x v /\ p.refine v})
+: action_except (v:a{compatible p x v /\ p.refine v})
     (pts_to' u#a u#b r x)
     (fun v -> pts_to' u#a u#b r (f v))
 
@@ -295,7 +323,7 @@ val write'
     (r:ref a p)
     (x y:Ghost.erased a)
     (f:FStar.PCM.frame_preserving_upd p x y)
-: action_except base_heap unit
+: action_except unit
     (pts_to' u#a u#b r x)
     (fun _ -> pts_to' u#a u#b r y)
 
@@ -305,9 +333,9 @@ val share'
     (r:ref a pcm)
     (v0:FStar.Ghost.erased a)
     (v1:FStar.Ghost.erased a{composable pcm v0 v1})
-: ghost_action_except base_heap unit
+: ghost_action_except unit
     (pts_to' u#a u#b r (v0 `op pcm` v1))
-    (fun _ -> pts_to' u#a u#b r v0 `base_heap.star` pts_to' u#a u#b r v1)
+    (fun _ -> pts_to' u#a u#b r v0 `star` pts_to' u#a u#b r v1)
 
 val gather'
     (#a:Type)
@@ -315,8 +343,8 @@ val gather'
     (r:ref a pcm)
     (v0:FStar.Ghost.erased a)
     (v1:FStar.Ghost.erased a)
-: ghost_action_except base_heap (squash (composable pcm v0 v1))
-    (pts_to' u#a u#b r v0 `base_heap.star` pts_to' u#a u#b r v1)
+: ghost_action_except (squash (composable pcm v0 v1))
+    (pts_to' u#a u#b r v0 `star` pts_to' u#a u#b r v1)
     (fun _ -> pts_to' u#a u#b r (op pcm v0 v1))
 
 val pts_to_not_null_action'
@@ -324,6 +352,14 @@ val pts_to_not_null_action'
       (#pcm:pcm a)
       (r:erased (ref a pcm))
       (v:Ghost.erased a)
-: ghost_action_except base_heap (squash (not (is_null r)))
+: ghost_action_except (squash (not (is_null r)))
     (pts_to' u#a u#b r v)
     (fun _ -> pts_to' u#a u#b r v)
+
+val lift_ghost
+      (#a:Type u#a)
+      (#p:slprop u#b)
+      (#q:a -> GTot slprop)
+      (ni_a:non_info a)
+      (f:erased (ghost_action_except a p q))
+: ghost_action_except a p q
